WIP implementation of QUIC.fst progressing towards the mythical switch

src/QUIC.fst
@@ -60,7 +60,7 @@ noeq type mstate_t i =
   reader: QModel.stream_reader writer ->
   ts: itraffic_secret i{derived reader ts} -> // FIXME erased
   mstate_t i
-  
+
 let istate_t i = QImpl.state i
 
 let state i =
@@ -72,12 +72,14 @@ let istate (#i:index{not I.model}) (s:state i) = s <: istate_t (iid i)
 
 let footprint #i h s =
   if I.model then
-    QModel.rfootprint (mstate s).reader
+    QModel.rfootprint (mstate s).reader `B.loc_union` QModel.footprint (mstate s).writer
   else QImpl.footprint h (istate s)
 
 let invariant #i h s =
   if I.model then
-    QModel.invariant (mstate s).writer h <: Type0
+    let Ideal writer reader _ = mstate s in
+    QModel.invariant writer h /\ QModel.rinvariant reader h /\
+    B.loc_disjoint (QModel.rfootprint (mstate s).reader) (QModel.footprint (mstate s).writer)
   else QImpl.invariant h (istate s)
 
 let g_traffic_secret #i s h =
@@ -86,12 +88,80 @@ let g_traffic_secret #i s h =
     QImpl.g_traffic_secret (B.deref h (istate s))
 
 let g_initial_packet_number #i s h =
-  if I.model then admit ()
+  if I.model then QModel.g_initial_packet_number #(mid i) (mstate s).writer
   else
-    QImpl.g_initial_packet_number (B.deref h (istate s)) h
+    QImpl.g_initial_packet_number (B.deref h (istate s))
 
 let g_last_packet_number #i s h =
   if I.model then
-    QModel.expected_pnT (mstate s).reader h
+    admit ()
   else
     QImpl.g_last_packet_number (B.deref h (istate s)) h
+
+// TODO: reveal in the interface (just for good measure)
+let frame_invariant #i l s h0 h1 =
+  if I.model then
+    let Ideal w r _ = mstate #(mid i) s in
+    QModel.frame_invariant w h0 l h1;
+    QModel.rframe_invariant r h0 l h1
+  else
+    QImpl.frame_invariant #(iid i) l s h0 h1
+
+/// Ingredients we need for the mythical switch
+
+/// First, a stateful equivalent of as_seq. Implementation doesn't need to be
+/// efficient.
+
+let rec as_seq #a (b: B.buffer a) (l: UInt32.t { l == B.len b }): Stack (S.seq a)
+  (requires fun h0 ->
+    B.live h0 b)
+  (ensures fun h0 r h1 ->
+    h0 == h1 /\
+    B.as_seq h0 b `S.equal` r)
+=
+  let h0 = ST.get () in
+  if l = 0ul then
+    S.empty
+  else
+    let hd = B.index b 0ul in
+    let l = l `U32.sub` 1ul in
+    let b = B.sub b 1ul l in
+    S.cons hd (as_seq b l)
+
+#set-options "--fuel 0 --ifuel 0 --z3rlimit 200"
+
+let encrypt #i s dst dst_pn h plain plain_len =
+  if I.model then
+    let i = i <: QModel.id in
+    // A pure version of plain suitable for calling specs with. From here on,
+    // this is a "magical" value that has no observable side-effects since it
+    // belongs to spec-land.
+    let plain_s = as_seq plain in
+
+    // We can clear out the contents of the "real" buffer.
+    B.fill plain 0uy plain_len;
+
+    // Yet do a "fake" call that generates the same side-effects.
+    push_frame ();
+    let hash_alg: QSpec.ha = I.ae_id_hash (fst i) in
+    let aead_alg = I.ae_id_info (fst i) in
+    let dummy_traffic_secret = B.alloca 0uy (Hacl.Hash.Definitions.hash_len hash_alg) in
+    let dummy_index: QImpl.index = { QImpl.hash_alg = hash_alg; QImpl.aead_alg = aead_alg } in
+    let dummy_dst = B.alloca B.null 1ul in
+    (*let dummy_cipher =
+      B.alloca 0uy (QImpl.header_len h `U32.add` plain_len `U32.add` Model.AEAD.tag_len)
+    in
+    let dummy_dst_pn = B.alloca 0UL 1ul in*)
+    let r = QImpl.create_in dummy_index HS.root dummy_dst 0UL dummy_traffic_secret in
+    assume (r <> UnsupportedAlgorithm);
+    let dummy_s = LowStar.BufferOps.(!* dummy_dst) in
+    admit (); // problem with header_live precondition, need to debug
+    let r = QImpl.encrypt #(G.hide dummy_index) dummy_s dst dst_pn h plain plain_len in
+    B.free dummy_s;
+    pop_frame ();
+
+    admit ();
+    r
+  else
+    let s = s <: QImpl.state i in
+    QImpl.encrypt #(G.hide (i <: QImpl.index)) s dst dst_pn h plain plain_len
